state/LabeledRefs.fst
@@ -30,11 +30,11 @@ let lemma_fresh_ref_not_shared = (fun #a #rel r h -> ())
 
 let lemma_unmodified_map_implies_same_shared_status (ms:Set.set nat) (h0 h1:heap) :
     Lemma (h0 `contains` secret_map /\ h0 `heap_rel` h1 /\ ~(addr_of secret_map `Set.mem` ms) /\ modifies ms h0 h1 ==>
-      (forall #a #rel (r:mref a rel). is_shared r h0 <==> is_shared r h1)) =
-    introduce h0 `contains` secret_map /\ h0 `heap_rel` h1 /\ ~(addr_of secret_map `Set.mem` ms) /\ modifies ms h0 h1 ==> (forall #a #rel (r:mref a rel). is_shared r h0 <==> is_shared r h1) with _. begin
-      introduce forall a rel (r:mref a rel). is_shared r h0 <==> is_shared r h1 with begin
-        introduce is_shared r h0 ==> is_shared r h1 with _. ();
-        introduce is_shared r h1 ==> is_shared r h0 with _. ()
+      (forall #a #rel (r:mref a rel). is_shareable r h0 <==> is_shareable r h1)) =
+    introduce h0 `contains` secret_map /\ h0 `heap_rel` h1 /\ ~(addr_of secret_map `Set.mem` ms) /\ modifies ms h0 h1 ==> (forall #a #rel (r:mref a rel). is_shareable r h0 <==> is_shareable r h1) with _. begin
+      introduce forall a rel (r:mref a rel). is_shareable r h0 <==> is_shareable r h1 with begin
+        introduce is_shareable r h0 ==> is_shareable r h1 with _. ();
+        introduce is_shareable r h1 ==> is_shareable r h0 with _. ()
       end
     end
 
